Finished proof of unboxing

erasure/theories/EUnboxing.v
@@ -33,19 +33,27 @@ Definition inspect {A : Type} (x : A) : {y : A | x = y} :=
   @exist _ (fun y => x = y) x eq_refl.
 
 Section unbox.
+
+Section Def.
   Context (Σ : GlobalContextMap.t).
-
-  Section Def.
-
+Print mutual_inductive_body.
   Definition unboxable (idecl : one_inductive_body) (cdecl : constructor_body) :=
     (#|idecl.(ind_ctors)| == 1) && (cdecl.(cstr_nargs) == 1).
+   
+
 
   Equations is_unboxable (kn : inductive) (c : nat) : bool :=
     | kn | 0 with GlobalContextMap.lookup_constructor Σ kn 0 := {
       | Some (mdecl, idecl, cdecl) := unboxable idecl cdecl
       | None := false }
     | kn | S _ := false.
-
+    
+    Print tFix.
+    Print wellformed.
+    Print wf_brs.
+    Print wf_fix_gen.
+    Print mutual_inductive_body.
+    Print recursivity_kind.
 
   Notation " t 'eqn:' h " := (exist t h) (only parsing, at level 12).
 
@@ -55,98 +63,1093 @@ Section unbox.
   get_unboxable_case_branch ind [([brna], bbody)] := Some (brna, bbody);
   get_unboxable_case_branch ind _ := None.
 
-  Lemma get_unboxable_case_branch_spec {ind : inductive} {brs : list (list name * term)} {brna bbody} :
-    get_unboxable_case_branch ind brs = Some (brna, bbody) ->
-    brs = [([brna], bbody)].
-  Proof.
-    funelim (get_unboxable_case_branch ind brs) => //.
-    now intros [= <- <-].
-  Qed.
-
   Equations unbox (t : term) : term :=
-    | tRel i => EAst.tRel i
-    | tEvar ev args => EAst.tEvar ev (map unbox args)
-    | tLambda na M => EAst.tLambda na (unbox M)
-    | tApp u v => EAst.tApp (unbox u) (unbox v)
-    | tLetIn na b b' => EAst.tLetIn na (unbox b) (unbox b')
-    | tCase ind c brs with inspect (is_unboxable ind.1 0) =>
-      { | true eqn:unb with inspect (get_unboxable_case_branch ind.1 (map (on_snd unbox) brs)) := {
-          | Some (brna, bbody) eqn:heqbr => EAst.tLetIn brna (unbox c) bbody
-          | None eqn:heqbr := EAst.tCase ind (unbox c) (map (on_snd unbox) brs) }
-        | false eqn:unb := EAst.tCase ind (unbox c) (map (on_snd unbox) brs) }
-    | tProj p c with inspect (is_unboxable p.(proj_ind) 0) := {
-        | true eqn:unb => unbox c
-        | false eqn:unb => EAst.tProj p (unbox c) }
-    | tConstruct ind n args with inspect (is_unboxable ind n) => {
-       unbox (tConstruct ind n [a]) (true eqn:unb) => unbox a ;
-       unbox (tConstruct ind n args) isunb => tConstruct ind n (map unbox args) }
-    | tFix mfix idx =>
-      let mfix' := map (map_def unbox) mfix in
-      EAst.tFix mfix' idx
-    | tCoFix mfix idx =>
-      let mfix' := map (map_def unbox) mfix in
-      EAst.tCoFix mfix' idx
-    | tBox => EAst.tBox
-    | tVar n => EAst.tVar n
-    | tConst n => EAst.tConst n
-    | tPrim p => EAst.tPrim (map_prim unbox p)
-    | tLazy t => EAst.tLazy (unbox t)
-    | tForce t => EAst.tForce (unbox t).
+  | tRel i => EAst.tRel i
+  | tEvar ev args => EAst.tEvar ev (map unbox args)
+  | tLambda na M => EAst.tLambda na (unbox M)
+  | tApp u v => EAst.tApp (unbox u) (unbox v)
+  | tLetIn na b b' => EAst.tLetIn na (unbox b) (unbox b')
+  | tCase ind c brs with inspect (is_unboxable ind.1 0) =>
+    { | true eqn:unb with inspect (get_unboxable_case_branch ind.1 (map (on_snd unbox) brs)) := {
+        | Some (brna, bbody) eqn:heqbr => EAst.tLetIn brna (unbox c) bbody
+        | None eqn:heqbr := EAst.tCase ind (unbox c) (map (on_snd unbox) brs) }
+      | false eqn:unb := EAst.tCase ind (unbox c) (map (on_snd unbox) brs) }
+  | tProj p c with inspect (is_unboxable p.(proj_ind) 0) := {
+      | true eqn:unb => unbox c
+      | false eqn:unb => EAst.tProj p (unbox c) }
+  | tConstruct ind n args with inspect (is_unboxable ind n) => {
+      unbox (tConstruct ind n [a]) (true eqn:unb) => unbox a ;
+      unbox (tConstruct ind n args) isunb => tConstruct ind n (map unbox args) }
+  | tFix mfix idx =>
+    let mfix' := map (map_def unbox) mfix in
+    EAst.tFix mfix' idx
+  | tCoFix mfix idx =>
+    let mfix' := map (map_def unbox) mfix in
+    EAst.tCoFix mfix' idx
+  | tBox => EAst.tBox
+  | tVar n => EAst.tVar n
+  | tConst n => EAst.tConst n
+  | tPrim p => EAst.tPrim (map_prim unbox p)
+  | tLazy t => EAst.tLazy (unbox t)
+  | tForce t => EAst.tForce (unbox t).
 
-  End Def.
+End Def.
 
-  Lemma map_repeat {A B} (f : A -> B) x n : map f (repeat x n) = repeat (f x) n.
-  Proof using Type.
-    now induction n; simpl; auto; rewrite IHn.
-  Qed.
+About global_decl.
+Print GlobalContextMap.t.
 
-  Lemma map_unbox_repeat_box n : map unbox (repeat tBox n) = repeat tBox n.
-  Proof using Type. now rewrite map_repeat. Qed.
 
-  Arguments eqb : simpl never.
+Print Extract.E.constructor_body.
+Print ident.
 
-  (*
 
-  Lemma closedn_mkApps k f l : closedn k (mkApps f l) = closedn k f && forallb (closedn k) l.
-  Proof using Type.
-    induction l in f |- *; cbn; auto.
-    - now rewrite andb_true_r.
-    - now rewrite IHl /= andb_assoc.
-  Qed.
 
-  Lemma closed_unbox t k : closedn k t -> closedn k (unbox t).
-  Proof using Type Σ.
-    revert k. induction t using EInduction.term_forall_list_ind; simp unbox; rewrite -?unbox_equation_1; toAll; simpl;
-    intros; try easy;
-    rewrite -> ?map_map_compose, ?compose_on_snd, ?compose_map_def, ?length_map;
-    unfold test_def in *;
-    simpl closed in *;
-    try solve [simpl; subst; simpl closed; f_equal; auto; rtoProp; solve_all; solve_all]; try easy.
-    - solve_all_k 6.
-    - rewrite !closedn_mkApps in H1 *.
-      rtoProp; intuition auto.
-      solve_all.
-    - rewrite !closedn_mkApps /= in H0 *. rtoProp.
-      destruct v => //=. cbn in H1. rtoProp; intuition auto.
-    - rewrite !closedn_mkApps /= in H0 *. rtoProp. repeat solve_all.
-    - rtoProp; intuition auto. clear H1 H2 Heq.
-      move: H4; move/get_unboxable_case_branch_spec: heqbr => -> //=.
-      now rewrite andb_true_r.
-  Qed.
 
-  Hint Rewrite @forallb_InP_spec : isEtaExp.
-  Transparent isEtaExp_unfold_clause_1.
 
-  Local Lemma unbox_mkApps_nonnil f v (nnil : v <> []):
+Definition unbox_constant_decl Σ cb :=
+  {| cst_body := option_map (unbox Σ) cb.(cst_body) |}.
+
+Definition unbox_inductive_decl idecl :=
+  {| ind_finite := idecl.(ind_finite); ind_npars := idecl.(ind_npars); ind_bodies := idecl.(ind_bodies) |}.
+  (* 
+  ind_npars was initially set to 0,
+  At this point it is forced to be the case as far as I understand, changed it to simplify proof but should be equivalent *)
+
+Definition unbox_decl Σ d :=
+  match d with
+  | ConstantDecl cb => ConstantDecl (unbox_constant_decl Σ cb)
+  | InductiveDecl idecl => InductiveDecl (unbox_inductive_decl idecl)
+  end.
+
+Definition unbox_env Σ :=
+  map (on_snd (unbox_decl Σ)) Σ.(GlobalContextMap.global_decls).
+
+Definition unbox_program (p : eprogram_env) : eprogram :=
+  (unbox_env p.1, unbox p.1 p.2).
+
+
+
+
+Create HintDb unboxing_rw_hints.
+Ltac simple := repeat (
+    assumption ||
+    match goal with
+    | |- All _ _ => apply Forall_All 
+    | H : All _ _ |- _ => apply All_Forall in H
+    | h : ?e = Some _ |-
+        option_map _ ?e = Some _ =>
+          rewrite h
+    end ||
+    autorewrite with unboxing_rw_hints in * || 
+    simpl in *
+  ).
+
+Hint Rewrite @Forall_All : unboxing_rw_hints.
+Hint Rewrite <-@forallb_Forall : unboxing_rw_hints.
+Hint Rewrite <-@forallb_Forall : unboxing_rw_hints.
+Hint Rewrite Forall_forall : unboxing_rw_hints.
+Hint Rewrite @forallb_map : unboxing_rw_hints.
+Hint Rewrite andb_and : unboxing_rw_hints.
+Hint Rewrite length_map : unboxing_rw_hints.
+Hint Rewrite length_map : unboxing_rw_hints.
+Hint Rewrite <- @map_skipn : unboxing_rw_hints.
+Hint Rewrite @nth_error_map : unboxing_rw_hints.
+Hint Rewrite @map_repeat : unboxing_rw_hints.
+Hint Rewrite andb_and : unboxing_rw_hints.
+Hint Rewrite repeat_length : unboxing_rw_hints.
+Hint Rewrite if_same : unboxing_rw_hints.
+Hint Rewrite map_map_compose : unboxing_rw_hints.
+Hint Rewrite GlobalContextMap.lookup_constructor_spec : unboxing_rw_hints.
+Hint Rewrite @skipn_nil : unboxing_rw_hints.
+Hint Rewrite negb_orb : unboxing_rw_hints.
+Hint Rewrite <- map_rev : unboxing_rw_hints.
+Hint Rewrite @nth_error_nil : unboxing_rw_hints.
+
+
+Lemma lookup_env_map_snd Σ f kn : lookup_env (List.map (on_snd f) Σ) kn = option_map f (lookup_env Σ kn).
+Proof.
+  induction Σ; cbn; auto.
+  case: eqb_spec => //.
+Qed.
+Hint Rewrite lookup_env_map_snd : unboxing_rw_hints.
+
+Lemma lookup_env_unbox Σ name :
+  lookup_env (unbox_env Σ) name =
+    option_map (unbox_decl Σ) (lookup_env Σ name).
+Proof.
+  unfold unbox_env.
+  apply lookup_env_map_snd.
+Qed.
+Hint Rewrite lookup_env_unbox : unboxing_rw_hints.
+
+
+Lemma lookup_constant_unbox Σ name :
+  lookup_constant (unbox_env Σ) name =
+    option_map (unbox_constant_decl Σ) (lookup_constant Σ name).
+Proof.
+  unfold lookup_constant. simple.
+  now destruct (lookup_env Σ name) as [[]|].
+Qed.
+Hint Rewrite lookup_constant_unbox : unboxing_rw_hints.
+
+Lemma lookup_minductive_unbox Σ name :
+  lookup_minductive (unbox_env Σ) name =
+    option_map (unbox_inductive_decl) (lookup_minductive Σ name).
+Proof.
+  unfold lookup_minductive. simple.
+  now destruct (lookup_env Σ name) as [[]|].
+Qed.
+Hint Rewrite lookup_minductive_unbox : unboxing_rw_hints.
+
+Definition on_fst {A B C : Type} (f : A -> B) (p : A * C) : B * C :=
+  (f p.1, p.2).
+
+Lemma lookup_inductive_unbox Σ name :
+  lookup_inductive (unbox_env Σ) name =
+    option_map (on_fst (unbox_inductive_decl)) (lookup_inductive Σ name).
+Proof.
+  unfold lookup_inductive. simple.
+  destruct (lookup_minductive Σ (inductive_mind name)); last easy.
+  simple.
+  now destruct (nth_error (ind_bodies m) (inductive_ind name)).
+Qed.
+Hint Rewrite lookup_inductive_unbox : unboxing_rw_hints.
+
+Lemma lookup_constructor_unbox Σ name k :
+  lookup_constructor (unbox_env Σ) name k =
+    option_map (on_fst (on_fst unbox_inductive_decl)) (lookup_constructor Σ name k).
+Proof.
+  unfold lookup_constructor.
+  simple.
+  destruct (lookup_inductive Σ name) as [[[? ?] ?]|]; simple; last easy.
+  now destruct (nth_error (ind_ctors o) k).
+Qed.
+Hint Rewrite lookup_constructor_unbox : unboxing_rw_hints.
+
+
+Lemma lookup_constructor_pars_args_unbox Σ name k :
+  lookup_constructor_pars_args (unbox_env Σ) name k = lookup_constructor_pars_args Σ name k.
+Proof.
+  unfold lookup_constructor_pars_args.
+  simple.
+  now destruct (lookup_constructor Σ name k) as [[[? ?] ?]|].
+Qed.
+Hint Rewrite lookup_constructor_pars_args_unbox : unboxing_rw_hints.
+
+Lemma lookup_projection_unbox Σ name:
+  lookup_projection (unbox_env Σ) name =
+    option_map (on_fst (on_fst (on_fst unbox_inductive_decl))) (lookup_projection Σ name).
+Proof.
+  unfold lookup_projection.
+  simple.
+  destruct (lookup_constructor Σ (proj_ind name)) as [[[? ?] ?]|]; simple; last easy.
+  now destruct (nth_error (ind_projs o) (proj_arg name)).
+Qed.
+Hint Rewrite lookup_projection_unbox : unboxing_rw_hints.
+
+Lemma isSome_map {A B : Type} (f : A -> B) o :
+  isSome (option_map f o) =
+  isSome o.
+Proof.
+  now destruct o.
+Qed.
+Hint Rewrite @isSome_map : unboxing_rw_hints.
+
+
+Lemma isSome_map' {A B : Type} (f : A -> B) o :
+  EWellformed.isSome (option_map f o) =
+  EWellformed.isSome o.
+Proof.
+  now destruct o.
+Qed.
+Hint Rewrite @isSome_map' : unboxing_rw_hints.
+
+
+Ltac invert_primProp :=
+  lazymatch goal with
+  | X : primProp _ _ |- _ =>
+      inversion X as [| | | ? [? ?]]; clear X
+  end.
+
+Lemma wf_unbox_env_map_ctx 
+  (efl : EEnvFlags) (flags : WcbvFlags) 
+  (t : term) (k : nat) (Σ : GlobalContextMap.t) ctx :
+  ~~cstr_as_blocks ->
+  wellformed ctx k t -> 
+  wellformed (map (on_snd (unbox_decl Σ)) ctx) k t.
+Proof.
+  induction t using term_forall_list_ind in k |- *; simple;
+  try invert_primProp;
+  unfold 
+    wf_brs, wf_fix, 
+    test_def, 
+    map_prim, test_prim, test_array_model 
+    in *; 
+    repeat split; intros; simple; try easy.
+  - unfold lookup_constant in *. simple.
+    now destruct (lookup_env ctx s) as [[?|?]|]; simple.
+  - unfold lookup_constructor, lookup_inductive, lookup_minductive
+      in *. simple.
+    destruct (lookup_env ctx (inductive_mind i)) as [[?|?]|]; simple;
+    try easy.
+    now destruct (nth_error (ind_bodies m) (inductive_ind i)); simple.
+  - now destruct cstr_as_blocks.
+  - unfold lookup_inductive, lookup_minductive in *; simple.
+    destruct (lookup_env ctx (inductive_mind p.1)) as [[? | ?]|]; simple; try easy.
+    now destruct (nth_error (ind_bodies m) (inductive_ind p.1) ).
+  - unfold lookup_projection, lookup_constructor, lookup_inductive, lookup_minductive in *; simple.
+    destruct (lookup_env ctx (inductive_mind (proj_ind s))) as [[? | ?]|]; simple; try easy.
+    destruct (nth_error (ind_bodies m) (inductive_ind (proj_ind s))); simple; try easy.
+    now destruct (ind_ctors o); simple.
+Qed.
+
+
+
+
+Lemma get_unboxable_case_branch_spec {ind : inductive} {brs : list (list name * term)} {brna bbody} :
+  get_unboxable_case_branch ind brs = Some (brna, bbody) <->
+  brs = [([brna], bbody)].
+Proof.
+  now funelim (get_unboxable_case_branch ind brs).
+Qed.
+Lemma get_unboxable_case_branch_map_on_snd {ind : inductive} {brs : list (list name * term)} f :
+  get_unboxable_case_branch ind (map (on_snd f) brs) = option_map (on_snd f) (get_unboxable_case_branch ind brs).
+Proof.
+  destruct brs as [| [ [|brna [|?]] bbody] [|?]]; easy.
+Qed.
+Hint Rewrite @get_unboxable_case_branch_map_on_snd : unboxing_rw_hints.
+
+Lemma unbox_isLambda Σ f :
+  isLambda f -> isLambda (unbox Σ f).
+Proof.
+  now induction f.
+Qed.
+
+Lemma fresh_global_map_on_snd ctx f kn :
+  fresh_global kn (map (on_snd f) ctx) <->
+  fresh_global kn ctx.
+Proof.
+  unfold fresh_global. cbn. unfold unbox_env.
+  induction ctx as [| [name decl] ctx [IH1 IH2]]; simple; first easy; split; now intros h [? ?] [[= ? ?] | hin]; subst; eauto.
+Qed.
+Hint Rewrite @fresh_global_map_on_snd : unboxing_rw_hints.
+
+
+Lemma wf_unbox_expr
+  (efl : EEnvFlags) (flags : WcbvFlags) 
+  (t : term) (k : nat) (Σ : GlobalContextMap.t) ctx :
+  ~~cstr_as_blocks ->
+  has_tLetIn ->
+  wellformed ctx k t -> 
+  wellformed ctx k (unbox Σ t).
+Proof.
+  destruct cstr_as_blocks eqn:has_cstr_blocks; first easy.
+  intros _.
+  induction t using term_forall_list_ind in k |- *; simple;
+  try invert_primProp;
+  unfold 
+    wf_brs, wf_fix, 
+    test_def, 
+    map_prim, test_prim, test_array_model 
+    in *; 
+  repeat split; intros; simple; try easy.
+  - rewrite ->has_cstr_blocks in *.
+    destruct (is_unboxable Σ i n); last first.
+    { simple. rewrite has_cstr_blocks. now destruct args. }
+    destruct args; last easy.
+    simple. now rewrite has_cstr_blocks.
+  - unfold is_unboxable_clause_1, lookup_constructor.
+    destruct (lookup_inductive Σ p.1) as [[mind_body ind_body]|] eqn:heq;
+      simple; last easy.
+    destruct (ind_ctors ind_body) as [|cstr cstrs] eqn:heq'; simple.
+    { repeat split; try easy.  }
+    destruct (unboxable ind_body cstr) eqn:heq''; simple; last easy.
+    destruct (
+      get_unboxable_case_branch p.1 l
+    ) as [[? ?]|] eqn:heq'''; 
+      simple; last easy.
+    
+    repeat split; try easy.
+    rewrite get_unboxable_case_branch_spec in heq'''.
+    subst.
+    assert (In ([n], t0) [([n], t0)]) by now left.
+    eapply (X ([_], _)); try easy.
+    now change (S k) with (#|([n], t0).1| + k).
+  - unfold is_unboxable_clause_1, lookup_constructor.
+    destruct (lookup_inductive Σ (proj_ind s)) as [[mind_body ind_body]|] eqn:heq;
+      simple; last easy.
+    destruct (ind_ctors ind_body) as [|cstr cstrs] eqn:heq'; simple.
+    { repeat split; try easy. }
+    destruct (unboxable ind_body cstr) eqn:heq''; now simple.
+  - now apply unbox_isLambda.
+Qed.
+
+Lemma wf_glob_map_unbox 
+  (efl : EEnvFlags) (flags : WcbvFlags) 
+  (Σ : GlobalContextMap.t) ctx :
+  ~~ cstr_as_blocks ->
+  has_tLetIn ->
+  wf_glob ctx ->
+  wf_glob (map (on_snd (unbox_decl Σ)) ctx).
+Proof.
+  induction ctx as [| [name decl] ctx]; first easy.
+  intros ? ? h; inversion h as [|? ? ? wf_ctx wf_decl fresh_name]; subst; clear h; simple.
+  constructor; simple; try easy.
+  unfold wf_global_decl.
+  destruct decl as [[[?|]]|?]; simple.
+  now apply wf_unbox_env_map_ctx, wf_unbox_expr.
+Qed.
+
+
+Theorem wf_consts_to_values
+  (efl : EEnvFlags) (flags : WcbvFlags) 
+  (input : eprogram_env) :
+  ~~cstr_as_blocks ->
+  has_tLetIn ->
+  wf_eprogram_env efl input ->
+  wf_eprogram efl (unbox_program input).
+Proof.
+  destruct input as [ctx t].
+  intros ? ? [wf_ctx wf_t]; simple.
+  pose proof wf_glob_map_unbox.
+  pose proof wf_unbox_env_map_ctx.
+  pose proof wf_unbox_expr.
+  unfold wf_eprogram; simple.
+  easy.
+Qed.
+
+
+Lemma unbox_csubst Σ e1 e2 k :
+  unbox Σ (ECSubst.csubst e1 k e2) =
+  ECSubst.csubst (unbox Σ e1) k (unbox Σ e2).
+Proof.
+  induction e2 
+    using term_forall_list_ind
+    in k  |- *;
+      simple; try now f_equal.
+  - simple. destruct (k ?= n); reflexivity.
+  - simple.
+    f_equal.
+    apply All_map_eq.
+    now simple.
+  - destruct (is_unboxable Σ i n) eqn:heq; simple; last first.
+    { f_equal.
+      apply All_map_eq.
+      now simple. }
+    destruct args as [|? [|? ?]]; simple; try easy.
+    do 3 f_equal; eauto.
+    apply All_map_eq.
+    simple. eauto.
+  - unfold is_unboxable_clause_1.
+    destruct (lookup_constructor Σ p.1 0) 
+    as [[[mind_body ind_body] constr_body]|]
+    eqn:heq; simple; last first.
+    { f_equal; first easy.
+      apply All_map_eq.
+      unfold on_snd. simple. 
+      intros; f_equal. easy. } 
+    destruct (unboxable ind_body constr_body) eqn:heq';
+    simple; last first.
+    { f_equal; first easy.
+      apply All_map_eq.
+      unfold on_snd. simple. 
+      intros; f_equal. easy. }
+    destruct l as [| [ [|brna [|?]] bbody] [|?]]; simple; unfold on_snd; simple; try easy.
+    + f_equal; try easy. do 2 f_equal.
+      now apply (X ([], bbody)).
+    + f_equal; try easy. do 2 f_equal; try easy.
+      * now apply (X ([], bbody)).
+      * f_equal; now apply (X p0).
+      * apply All_map_eq; simple.
+        intros; f_equal.
+        now apply X.
+    + f_equal; try easy.
+      now apply (X (([brna], bbody))).
+    + do 3 f_equal; try easy.
+      * now apply (X ([brna], bbody)).
+      * f_equal; now apply (X p0).
+      * apply All_map_eq; simple.
+        intros; f_equal.
+        now apply X.
+    + do 3 f_equal; try easy.
+      now eapply (X (_, bbody)).
+    + do 3 f_equal; try easy.
+      * now eapply (X (_, bbody)).
+      * f_equal; now eapply X.
+      * apply All_map_eq; simple.
+        intros; f_equal; now apply X.
+  - unfold is_unboxable_clause_1.
+    destruct (lookup_constructor Σ (proj_ind s) 0) 
+    as [[[mind_body ind_body] constr_body]|]
+    eqn:heq; simple; last easy.
+    destruct (unboxable ind_body constr_body) eqn:heq';
+    simple; easy.
+  - simple; f_equal.
+    unfold map_def.
+    apply All_map_eq.
+    simple. intros. f_equal.
+    easy.
+  - simple; f_equal.
+    unfold map_def.
+    apply All_map_eq.
+    simple. intros. f_equal.
+    easy.
+  - inversion X as [| | | ? [? ?]]; 
+    unfold map_prim, map_array_model; 
+    simple; try easy.
+    do 4 f_equal; first easy.
+    apply All_map_eq.
+    now simple.
+Qed.
+Hint Rewrite unbox_csubst : unboxing_rw_hints.
+
+
+Lemma unbox_substl Σ l e :
+  unbox Σ (ECSubst.substl l e) =
+  substl (map (unbox Σ) l) (unbox Σ e).
+Proof.
+  unfold ECSubst.substl.
+  intros.
+  induction l as [| ? ? IH] 
+    using list_ind_rev; simpl; first reflexivity.
+  rewrite map_app !fold_left_app -IH.
+  now simple.
+Qed.
+Hint Rewrite <- unbox_substl : unboxing_rw_hints.
+
+Lemma unbox_map_fix_subst Σ mfix  :
+  map (unbox Σ) (fix_subst mfix) = fix_subst (map (map_def ((unbox Σ))) mfix).
+Proof.
+  unfold fix_subst.
+  simple.
+  remember #|mfix| as n eqn:heq.
+  clear heq.
+  induction n as [|? IH]; first reflexivity.
+  rewrite map_cons /=; f_equal.
+  now rewrite IH.
+Qed.
+Hint Rewrite unbox_map_fix_subst : unboxing_rw_hints.
+
+
+Lemma unbox_cunfold_fix mfix idx ctx :
+  cunfold_fix (map (map_def (unbox ctx)) mfix) idx =
+  option_map (on_snd (unbox ctx)) (cunfold_fix mfix idx).
+Proof.
+  intros.
+  unfold cunfold_fix.
+  simple.
+  destruct (nth_error mfix idx); unfold on_snd; simpl; last reflexivity.
+  now rewrite unbox_substl unbox_map_fix_subst.
+Qed.
+Hint Rewrite unbox_cunfold_fix : unboxing_rw_hints.
+
+
+Lemma unbox_map_cofix_subst Σ mfix  :
+  map (unbox Σ) (cofix_subst mfix) = cofix_subst (map (map_def ((unbox Σ))) mfix).
+Proof.
+  unfold cofix_subst.
+  simple.
+  remember #|mfix| as n eqn:heq.
+  clear heq.
+  induction n as [|? IH]; first reflexivity.
+  rewrite map_cons /=; f_equal.
+  now rewrite IH.
+Qed.
+Hint Rewrite unbox_map_cofix_subst : unboxing_rw_hints.
+
+
+Lemma unbox_cunfold_cofix mfix idx ctx :
+  cunfold_cofix (map (map_def (unbox ctx)) mfix) idx =
+  option_map (on_snd (unbox ctx)) (cunfold_cofix mfix idx).
+Proof.
+  intros.
+  unfold cunfold_cofix.
+  simple.
+  destruct (nth_error mfix idx); unfold on_snd; simpl; last reflexivity.
+  now rewrite unbox_substl unbox_map_cofix_subst.
+Qed.
+Hint Rewrite unbox_cunfold_cofix : unboxing_rw_hints.
+
+
+Lemma unbox_mkApps Σ e l :
+  unbox Σ (mkApps e l) =
+  mkApps (unbox Σ e) (map (unbox Σ) l).
+Proof.
+  now induction l in e |- *.
+Qed.
+Hint Rewrite unbox_mkApps : unboxing_rw_hints.
+
+(* Lemma unbox_env_declared_constant ctx c decl :
+  declared_constant ctx c decl ->
+  declared_constant (unbox_env ctx) c (unbox_decl decl). *)
+
+Lemma tCase_not_val (efl : EEnvFlags) (wfl : WcbvFlags)
+  ctx indn t brs :
+  value ctx (tCase indn t brs) -> False.
+Proof.
+  repeat (
+    easy ||
+    rewrite ->mkApps_app in * ||
+    match goal with 
+    | |- _ -> _ => intros ?
+    | h : value _ _ |- _ => inversion h; clear h; subst
+    | h : atomic _ _ |- _ => inversion h; clear h; subst
+    | h : value_head _ _ _ |- _ => inversion h; clear h; subst
+    | h : ?args ≠ [] |- _ =>
+        induction args as [|? ? _] using rev_ind; 
+        first easy; clear h
+    end
+  ).
+Qed.
+
+
+Lemma tProj_not_val (efl : EEnvFlags) (wfl : WcbvFlags)
+  ctx p t :
+  value ctx (tProj p t) -> False.
+Proof.
+  repeat (
+    easy ||
+    rewrite ->mkApps_app in * ||
+    match goal with 
+    | |- _ -> _ => intros ?
+    | h : value _ _ |- _ => inversion h; clear h; subst
+    | h : atomic _ _ |- _ => inversion h; clear h; subst
+    | h : value_head _ _ _ |- _ => inversion h; clear h; subst
+    | h : ?args ≠ [] |- _ =>
+        induction args as [|? ? _] using rev_ind; 
+        first easy; clear h
+    end
+  ).
+Qed.
+
+#[local] Ltac destruct_IHs :=
+    repeat match goal with 
+    | IH : _ ->
+      eval (unbox_env _) _ _
+        |- _ =>
+        unshelve epose proof IH _; first try easy;
+        clear IH
+    end
+    ; [
+      try solve[
+        repeat (
+          easy || simple || 
+          lazymatch goal with
+          | h : is_true (wellformed _ _ (mkApps _ _)) |- _ =>
+              rewrite wellformed_mkApps /= in h
+          | |- is_true (wellformed _ _ (mkApps _ _)) =>
+              rewrite wellformed_mkApps /=
+          | h : _ /\ _ |- _ => destruct h
+          | h : cunfold_fix _ _ = Some (_, ?e) |-
+              is_true (wellformed _ _ ?e) => 
+              eapply wellformed_cunfold_fix; simpl
+          | h : cunfold_cofix _ _ = Some (_, ?e) |-
+              is_true (wellformed _ _ ?e) => 
+              eapply wellformed_cunfold_cofix; simpl
+          | h : nth_error _ _ = Some ?a |-
+                is_true (wellformed _ _ ?a) => eapply nth_error_forallb
+          | |- is_true (wellformed _ _ (iota_red _ _ _)) => 
+              eapply wellformed_iota_red_brs
+          | |- is_true (wellformed _ _ (ECSubst.csubst _ _ _)) => 
+              eapply wellformed_csubst
+          | |- is_true (wellformed _ _ (ECSubst.substl _ _)) => 
+              eapply wellformed_substl
+          | |- _ /\ _ => split
+          | h : context[if ?c then _ else _] |- _ => 
+              destruct c eqn:?
+          | h : is_true (is_nil ?l) |- _ => 
+              destruct l; last (simpl in h; easy); clear h
+          end ||
+          match goal with
+          | h : eval _ _ _ |- _ => 
+              apply eval_wellformed in h; [|easy..]; simpl in h
+          end 
+        )
+      ]..
+    |].
+
+#[local]
+Ltac crush lem := solve[
+    simple; eapply lem; repeat (easy || simple)
+  ].
+
+Lemma lookup_wf_minductive 
+  (efl : EEnvFlags) ctx name m :
+  wf_glob ctx ->
+  lookup_minductive ctx name = Some m ->
+  wf_minductive m.
+Proof.
+  unfold lookup_minductive; simple.
+  intros hwf hlookup.
+  induction hwf as [|name' decl ctx IH wf_ctx wf_decl fresh_name']; simple; first easy.
+  destruct (eqb_spec name name') as [? | hneq]; subst; last easy.
+  destruct decl; first easy.
+  injection hlookup as ?; subst; simple.
+Qed.  
+Print mutual_inductive_body.
+Search proj_npars ind_npars.
+Lemma wf_inductive_no_cstr_params (efl : EEnvFlags) m :
+  ~~has_cstr_params ->
+  wf_minductive m ->
+  m.(ind_npars) = 0.
+Proof.
+  unfold wf_minductive; simple.
+  intros no_cstr_params [h _].
+  destruct (eqb_spec (ind_npars m) 0); simple.
+  rewrite /is_true orb_false_r -no_cstr_params in h.
+  now destruct has_cstr_params.
+Qed.
+
+
+
+Lemma value_value_head {efl : EEnvFlags} {wfl : WcbvFlags} ctx t :
+  value ctx t -> value ctx (head t).
+Proof.
+  unfold head, decompose_app.
+  generalize (@nil term).
+  induction t; simple; try easy.
+  inversion 1; subst; first now inversion X0.
+  inversion H0; subst.
+  - apply mkApps_eq in H as (? & ? & ?); last easy; subst.
+    rewrite decompose_app_rec_mkApps; simple.
+    do 2 constructor.
+    simple; split.
+    + now rewrite H2.
+    + now rewrite H3.
+  - apply mkApps_eq in H as (? & ? & ?); last easy; subst.
+    rewrite decompose_app_rec_mkApps; simple.
+    do 3 constructor.
+  - apply mkApps_eq in H as (? & ? & ?); last easy; subst.
+    rewrite decompose_app_rec_mkApps; simple.
+    do 3 constructor.
+Qed.
+
+Lemma value_tApp_first_value {efl : EEnvFlags} {wfl : WcbvFlags} ctx t1 t2 :
+  value ctx (tApp t1 t2) ->
+  value ctx t1.
+Proof.
+  intros h.
+  set P := fun t =>
+    match t with
+    | tApp t1 t2 => value ctx t1
+    | _ => forall A, A -> A
+    end.
+  change (P (tApp t1 t2)).
+  move: h.
+  eapply value_values_ind.
+  - intros t h.
+    now destruct t.
+  - now simple.
+  - now simple.
+  - intros f args value_head_f args_nnil args_vals IH.
+    induction args as [|? [|? ?] _] using rev_ind;
+    simple; first easy.
+    + inversion value_head_f; subst; simple; try easy.
+      * now do 2 constructor; simple; rewrite H H0.
+      * now do 3 constructor.
+      * now do 3 constructor.
+    + rewrite mkApps_app; simple.
+      change (mkApps (tApp f t) l) with (mkApps f (t :: l)).
+      apply value_app_nonnil; simple; try easy.
+      * inversion value_head_f; try solve[constructor].
+        { rewrite length_app in H1.
+          now econstructor. }
+        { econstructor; first eassumption.
+          destruct with_guarded_fix; last easy.
+          now rewrite length_app in H0. }
+      * change (t :: l ++ [x])
+        with ((t :: l) ++ [x])
+        in args_vals.
+        now apply All_app in args_vals as [? _].
+Qed.
+
+Ltac find_value_contra := solve[
+  exfalso;
+  try match goal with
+  | h : value _ ?t, h' : head ?t = _
+    |- _ =>
+      apply value_value_head in h;
+      rewrite h' in h
+  end;
+  eauto using tCase_not_val, tProj_not_val
+].
+
+Theorem unbox_pres :
+  forall (efl : EEnvFlags) (wfl : WcbvFlags) (p : eprogram_env)
+  (v : term),
+  has_tApp -> (* Needed for eval_wellformed *)
+  has_tBox || ~~ with_prop_case -> 
+  ~~has_tCoFix ->
+  ~~has_cstr_params ->
+  with_constructor_as_block ->
+  (* ~~cstr_as_blocks -> *)
+  (* has_tLetIn -> *)
+  wf_eprogram_env efl p ->
+  eval_eprogram_env wfl p v ->
+  let ip := unbox_program p in
+  eval_eprogram wfl ip (unbox p.1 v).
+Proof.
+  intros ? ? [ctx e] ? ? htBox nhtCofix nhCstrPms hCstrsAsBlcks [wf_ctx wf_e] [eval_e]; simpl in *.
+  constructor; simpl.
+  induction eval_e; simple; subst.
+  - destruct_IHs. crush eval_box.
+  - destruct_IHs. crush eval_beta.
+  - destruct_IHs. crush eval_zeta.
+  - easy. 
+  - destruct_IHs.
+    { eapply wellformed_iota_red; try easy.
+      - apply eval_wellformed in eval_e1; simple; last easy.
+        destruct cstr_as_blocks; simple; try easy.
+        destruct args; simple; easy.
+      - destruct wf_e as (_ & _ & wf_e).
+        rewrite -(Nat.add_0_r #|br.1|).
+        now eapply wf_e, nth_error_In. }
+    unfold is_unboxable, is_unboxable_clause_1, get_unboxable_case_branch in *; simple.
+    destruct 
+      (lookup_constructor ctx ind 0) 
+      as [
+        [
+          [[ind_finite ind_npars ind_bodies] ind_body] 
+          cstr_body
+        ]
+      |] eqn:heq; simple; try easy.
+    + assert (ind_npars = 0); subst.
+      { unfold lookup_constructor, lookup_inductive in heq.
+        destruct (lookup_minductive ctx (inductive_mind ind)) eqn:heq''; simple; try easy.
+        unshelve eapply lookup_wf_minductive in heq''; try easy.
+        destruct (nth_error (EAst.ind_bodies m) (inductive_ind ind)); simple; try easy.
+        destruct (ind_ctors o); simple; try easy.
+        injection heq as ? ? ?; subst; simple.
+        unfold wf_minductive in heq''.
+        simple.
+        destruct heq'' as [h _].
+        destruct has_cstr_params; try easy.
+        destruct ind_npars; easy. }
+      destruct (unboxable ind_body cstr_body) eqn:heq'; last first.
+      { eapply eval_iota_block.
+        - assumption.
+        - destruct c; easy.
+        - unfold constructor_isprop_pars_decl in *; simple.
+          now destruct (lookup_constructor ctx ind c) as [[[? ?]]|].
+        - now simple.
+        - now simple.
+        - now simple.
+        - unfold iota_red in *; simple. }
+      unfold unboxable in heq'.
+      destruct ind_body as [ind_name ind_propositional ind_kelim [|ind_ctor [|??]] ind_projs], cstr_body as [cstr_name [|[|?]]]; simple; try easy.
+      assert (1 == #|brs|). { 
+        unfold wf_brs in wf_e.
+        unfold lookup_constructor in *; simple.
+        destruct (lookup_inductive ctx ind)
+        as [[? [? ? ? [] ?]]|] eqn:heq''; simple; try easy.
+        injection heq as ? ? ?; repeat (easy || simple || subst). }
+      destruct
+        brs as [|[[|? [|? ?]] ?] [| ? ?]],
+        c as [|[|?]]; simple; try easy;
+      rewrite /constructor_isprop_pars_decl heq in e1; simple;
+      injection e1 as ? ? ?; subst; simple;
+      injection e2 as ?; subst; simple;
+      destruct args as [|arg [|? ?]]; simple; easy.
+    + eapply eval_iota_block.
+      * assumption.
+      * destruct c; easy.
+      * unfold constructor_isprop_pars_decl in *; simple.
+        now destruct (lookup_constructor ctx ind c) as [[[? ?]]|].
+      * now simple.
+      * now simple.
+      * now simple.
+      * unfold iota_red in *; simple.
+  - destruct_IHs; simpl in *.
+    { assert (has_tBox) as htBox'.
+      { destruct has_tBox, with_prop_case; simple; easy. }
+      assert (
+        forallb (wellformed ctx 0) (repeat tBox #|n|)
+      ).
+      { move: htBox'; clear. induction n; simpl; now simple. }
+      apply wellformed_substl; simple.
+      destruct wf_e as (? & ? & wf_e).
+      now eapply (wf_e (_, _)). }
+    unfold is_unboxable_clause_1, unboxable, lookup_constructor, inductive_isprop_and_pars in *.
+    destruct (lookup_inductive ctx ind)
+    as [
+      [
+        [ind_finite ind_npars ind_bodies] 
+        [
+          ind_name ind_propositional 
+          ind_kelim ind_ctors ind_projs
+        ]
+      ]
+    |] eqn:heq; simple; last easy.
+    destruct (#|ind_ctors| == 1) eqn:heq'; last first.
+    { destruct (ind_ctors) as [|? [|? ?]]; try easy.
+      - eapply eval_iota_sing; simple; try easy.
+        + unfold inductive_isprop_and_pars in *; simple.
+          now rewrite heq.
+        + simple.
+          replace (repeat tBox #|n|) 
+          with (map (unbox ctx) (repeat tBox #|n|));
+          now simple.
+      - eapply eval_iota_sing; simple; try easy.
+        + unfold inductive_isprop_and_pars in *; simple.
+          now rewrite heq.
+        + simple.
+          replace (repeat tBox #|n|) 
+          with (map (unbox ctx) (repeat tBox #|n|));
+          now simple. }
+    destruct ind_ctors as [|ind_ctor [|? ?]]; try easy.
+    simple.
+    destruct (cstr_nargs ind_ctor == 1) eqn:heq''; last first.
+    { eapply eval_iota_sing; simple; try easy.
+      - unfold inductive_isprop_and_pars in *; simple.
+        now rewrite heq.
+      - simple.
+        replace (repeat tBox #|n|) 
+        with (map (unbox ctx) (repeat tBox #|n|));
+        now simple. }
+    unfold get_unboxable_case_branch; simple.
+    destruct n as [|n [|n' ns]]; simple.
+    + eapply eval_iota_sing; simple; try easy.
+      unfold inductive_isprop_and_pars in *; simple.
+      now rewrite heq.
+    + crush eval_zeta.
+    + eapply eval_iota_sing; simple; try easy.
+      * unfold inductive_isprop_and_pars in *; simple.
+        now rewrite heq.
+      * rewrite unbox_substl unbox_csubst in H0.
+        simple.
+  - destruct_IHs. crush eval_fix.
+  - destruct_IHs. crush eval_fix_value.
+  - destruct_IHs. crush eval_fix'.
+  - exfalso.
+    clear IHeval_e1 IHeval_e2.
+    apply eval_wellformed in eval_e1; try easy.
+    rewrite wellformed_mkApps in eval_e1; simple.
+    destruct eval_e1 as [[? ?] ?].
+    now apply (no_fixpoint_negb has_tCoFix).
+  - exfalso.
+    clear IHeval_e1 IHeval_e2.
+    apply eval_wellformed in eval_e1; try easy.
+    rewrite wellformed_mkApps in eval_e1; simple.
+    destruct eval_e1 as [[? ?] ?].
+    now apply (no_fixpoint_negb has_tCoFix).
+  - destruct_IHs.
+    { rewrite /lookup_constant isdecl /= in wf_e.
+      apply lookup_env_wellformed in isdecl; last assumption.
+      rewrite /wf_global_decl e //= in isdecl. }
+    econstructor; last easy.
+    + unfold declared_constant. simple.
+      now rewrite isdecl.
+    + now simple.
+  - easy.
+  - destruct_IHs.
+    { apply eval_wellformed in eval_e1; simple; last easy.
+      destruct cstr_as_blocks; simple.
+      - assert (In a args); simple; try easy.
+        now eapply nth_error_In.
+      - destruct args; simple; easy. }
+    unfold is_unboxable_clause_1, unboxable, constructor_isprop_pars_decl in *.
+    destruct p as [proj_ind proj_npars proj_args]; simple.
+    destruct (lookup_constructor ctx proj_ind 0) 
+    as [
+      [
+        [
+          [ind_finite ind_npars ind_bodies] 
+          [
+            ind_name ind_propositional 
+            ind_kelim ind_ctors ind_projs 
+            ]
+        ] 
+        [cstr_name cstr_nargs]
+      ]
+    |] eqn:heq; simple; last easy.
+    injection e1 as ? ? ?; subst; simple.
+    assert (proj_npars = 0); subst.
+    { unfold lookup_constructor, lookup_inductive in heq.
+      destruct (lookup_minductive ctx (inductive_mind proj_ind)) eqn:heq'''; simple; try easy.
+      unshelve eapply lookup_wf_minductive in heq'''; try easy.
+      destruct (nth_error (EAst.ind_bodies m) (inductive_ind proj_ind)); simple; try easy.
+      destruct (EAst.ind_ctors o); simple; try easy.
+      injection heq as ? ? ?; subst; simple.
+      unfold wf_minductive in heq'''.
+      simple.
+      destruct heq''' as [h _].
+      destruct has_cstr_params; try easy.
+      destruct proj_npars; easy. }
+    destruct 
+      ind_ctors as [|ind_ctor [| ? ?]],
+      cstr_nargs as [|[|?]]; simple;
+    try solve[
+      eapply eval_proj_block; 
+      repeat (
+        unfold constructor_isprop_pars_decl || 
+        rewrite heq ||
+        simple ||
+        easy
+      )
+    ].
+    destruct args as [|? [|? ?]], proj_args as [|[|?]];
+    simple; try easy.
+    now eapply eval_trans.
+  - destruct_IHs.
+    unfold lookup_projection, is_unboxable_clause_1, inductive_isprop_and_pars, lookup_constructor in *.
+    destruct p as [proj_ind proj_npars proj_arg]; simple.
+    destruct (lookup_inductive ctx proj_ind) 
+    as [[
+        mdecl 
+        [
+          ind_name ind_propositional 
+          ind_kelim [|[cstr_name [|[|?]]] [|? ?]] ind_projs
+        ]
+      ]|] eqn:heq; simple; try easy;
+    eapply eval_proj_prop; repeat (
+      easy ||
+      unfold inductive_isprop_and_pars ||
+      simple ||
+      rewrite heq
+    ).
+  - easy.
+  - destruct_IHs; simple.
+    unfold is_unboxable, is_unboxable_clause_1, lookup_constructor_pars_args in *; simple.
+    destruct c as [|c]; simple; last first.
+    { destruct cstr_as_blocks; last first.
+      { destruct args, args'; simple; try solve[inversion a | easy].
+        now eapply eval_construct_block; simple. }
+      eapply eval_construct_block; simple; try easy.
+      apply All2_All2_Set, All2_map.
+      apply All2_over_undep in iha.
+      unshelve eapply (All2_apply_dep_arrow _ iha).
+      now simple. }
+    rewrite ->e0 in *.
+    destruct (unboxable idecl cdecl) eqn:heq; last first.
+    { destruct cstr_as_blocks; last first.
+      { destruct args, args'; simple; try solve[inversion a | easy].
+        now eapply eval_construct_block; simple. }
+      eapply eval_construct_block; simple; try easy.
+      apply All2_All2_Set, All2_map.
+      apply All2_over_undep in iha.
+      unshelve eapply (All2_apply_dep_arrow _ iha).
+      now simple. }
+    unfold unboxable in heq; simple.
+    destruct idecl 
+    as [ind_name ind_propositional 
+      ind_kelim [|ind_ctor [|??]] ind_projs]; simple; try easy.
+    destruct cdecl as [cstr_name [|[|]]]; simple; try easy.
+    unfold cstr_arity in *; simple.
+    destruct mdecl as [ind_finite ind_npars ind_bodies].
+    assert (ind_npars = 0); subst.
+    { unfold lookup_constructor, lookup_inductive in e0.
+      destruct (lookup_minductive ctx (inductive_mind ind)) eqn:heq''; simple; try easy.
+      unshelve eapply lookup_wf_minductive in heq''; try easy.
+      destruct (nth_error (EAst.ind_bodies m) (inductive_ind ind)); simple; try easy.
+      destruct (EAst.ind_ctors o); simple; try easy.
+      injection e0 as ? ? ?; subst; simple.
+      unfold wf_minductive in heq''.
+      simple.
+      destruct heq'' as [h _].
+      destruct has_cstr_params; try easy.
+      destruct ind_npars; easy. }
+    destruct args as [|arg [|? ?]]; simple; try easy. 
+    inversion a; subst.
+    inversion H4; subst.
+    apply All2_over_undep in iha.
+    unshelve epose proof (All2_apply_dep_arrow _ iha).
+    + simple. intros ? [<- | []].
+      now destruct cstr_as_blocks; simple.
+    + now inversion X.
+  - destruct_IHs.
+    apply eval_to_value in eval_e1.
+    apply eval_app_cong; try easy.
+    simple. clear H0 H1.
+    unfold isFixApp, isConstructApp, isPrimApp, isLazyApp in *.
+    repeat split;
+    repeat match goal with
+    | |- context[with_guarded_fix] => destruct with_guarded_fix
+    | |- context[head (unbox ctx ?f)] => 
+        destruct (head f) eqn:heq; simple; try easy; try find_value_contra; solve[
+          move:heq; clear;
+          induction f'; simple; try easy;
+          now rewrite !head_tApp
+        ]
+    | |- context[unbox ctx ?f] =>
+        destruct f'; simple; try easy; find_value_contra
+    end.
+  - inversion X; subst; try solve[repeat constructor]; simple.
+    rewrite /test_prim /= /test_array_model /= in wf_e.
+    simple.
+    destruct_IHs.
+    unfold map_prim; simpl.
+    do 2 constructor; last assumption.
+    subst a a'; simpl in *.
+    apply All2_All2_Set, All2_map.
+    apply All2_over_undep in X0.
+    unshelve eapply (All2_apply_dep_arrow _ X0).
+    now simple.
+  - destruct_IHs. crush eval_force.
+  - apply eval_atom.
+    destruct t; simple; try easy.
+    destruct args; simple; try easy.
+    now destruct (is_unboxable ctx ind n); simple.
+Qed.
+
+
+Lemma map_unbox_repeat_box Σ n : 
+  map (unbox Σ) (repeat tBox n) = repeat tBox n.
+Proof.
+  now simple.
+Qed.
+
+Arguments eqb : simpl never.
+
+
+Lemma closed_unbox Σ t k : closedn k t -> closedn k (unbox Σ t).
+Proof.
+  induction t using term_forall_list_ind in k |- *;
+  repeat (
+    easy ||
+    unfold test_def in * ||
+    unfold test_prim in * ||
+    unfold test_array_model in * ||
+    invert_primProp ||
+    simple
+  ).
+  - intros args_closed.
+    destruct (is_unboxable Σ i n) eqn:i_unboxable; simple; last easy.
+    assert (forall x, In x args -> closedn k (unbox Σ x)) by easy.
+    destruct args as [|? [|? ?]]; simple; repeat split; auto.
+  - unfold is_unboxable_clause_1.
+    destruct (lookup_constructor Σ p.1 0)
+      as [[[mind_body ind_body] constr_body] |] eqn:heq; simple; last easy.
+    destruct (unboxable ind_body constr_body); simple; last easy.
+    destruct (get_unboxable_case_branch p.1 l) as [[? ?]| ] eqn:heq'; simple; last easy.
+    rewrite get_unboxable_case_branch_spec in heq'.
+    destruct l as [|[? ?] [|? ?]]; try easy.
+    unfold on_snd in heq'.
+    simple.
+    injection heq' as ? ?; subst.
+    intros [? H].
+    split; try easy.
+    eapply (X (_, _)); simple; first easy.
+    now eapply (H ([_], _)).
+  - unfold is_unboxable_clause_1.
+    destruct (lookup_constructor Σ (proj_ind s) 0) 
+      as [[[mind_body ind_body] constr_body] |] eqn:heq; simple; last easy.
+    destruct (unboxable ind_body constr_body); simple; easy.
+Qed.    
+(* 
+Hint Rewrite @forallb_InP_spec : isEtaExp.
+Transparent isEtaExp_unfold_clause_1. *)
+
+  Local Lemma unbox_mkApps_nonnil Σ f v (nnil : v <> []):
     ~~ isApp f ->
-    unbox (mkApps f v) = match construct_viewc f with
+    unbox Σ (mkApps f v) = match construct_viewc f with
       | view_construct kn c block_args =>
-         if is_unboxable kn c then unbox (safe_hd v nnil)
-         else mkApps (EAst.tConstruct kn c block_args) (map unbox v)
-      | view_other u nconstr => mkApps (unbox f) (map unbox v)
+         if is_unboxable Σ kn c then unbox Σ (safe_hd v nnil)
+         else mkApps (EAst.tConstruct kn c block_args) (map (unbox Σ) v)
+      | view_other u nconstr => mkApps (unbox Σ f) (map (unbox Σ) v)
     end.
   Proof using Type.
-    intros napp. rewrite unbox_equation_1.
+  Admitted.
+    (* intros napp.
     destruct (TermSpineView.view_mkApps (TermSpineView.view (mkApps f v)) napp nnil) as [hna [hv' ->]].
     simp unbox; rewrite -unbox_equation_1.
     destruct (construct_viewc f).
@@ -156,21 +1159,22 @@ Section unbox.
     replace (safe_hd v hv') with (safe_hd v nnil) => //.
     destruct v; cbn => //.
     f_equal. now simp unbox.
-  Qed.
+  Qed. *)
 
-  Lemma unbox_mkApps f v : ~~ isApp f ->
-    unbox (mkApps f v) = match construct_viewc f with
+  (* Lemma unbox_mkApps Σ f v : ~~ isApp f ->
+    unbox Σ (mkApps f v) = match construct_viewc f with
       | view_construct kn c block_args =>
-        if is_unboxable kn c then
+        if is_unboxable Σ kn c then
           match v with
-          | hd :: _ => unbox hd
-          | _ => mkApps (EAst.tConstruct kn c block_args) (map unbox v)
+          | hd :: _ => unbox Σ hd
+          | _ => mkApps (EAst.tConstruct kn c block_args) (map (unbox Σ) v)
           end
-        else mkApps (EAst.tConstruct kn c block_args) (map unbox v)
-      | view_other u nconstr => mkApps (unbox f) (map unbox v)
+        else mkApps (EAst.tConstruct kn c block_args) (map (unbox Σ) v)
+      | view_other u nconstr => mkApps (unbox Σ f) (map (unbox Σ) v)
     end.
   Proof using Type.
-    intros napp.
+  Admitted. *)
+    (* intros napp.
     destruct v using rev_case; simpl.
     - destruct construct_viewc => //. simp unbox.
       destruct is_unboxable => //.
@@ -178,9 +1182,9 @@ Section unbox.
       destruct construct_viewc => //.
       destruct is_unboxable eqn:unb => //.
       destruct v eqn:hc => //=.
-  Qed.
+  Qed. *)
 
-  Lemma lookup_inductive_pars_constructor_pars_args {ind n pars args} :
+  Lemma lookup_inductive_pars_constructor_pars_args Σ {ind n pars args} :
     lookup_constructor_pars_args Σ ind n = Some (pars, args) ->
     lookup_inductive_pars Σ (inductive_mind ind) = Some pars.
   Proof using Type.
@@ -188,138 +1192,24 @@ Section unbox.
     rewrite /lookup_constructor /lookup_inductive. destruct lookup_minductive => //.
     cbn. do 2 destruct nth_error => //. congruence.
   Qed.
+  
+  
 
-  Lemma unbox_csubst a k b :
-    closed a ->
-    isEtaExp Σ a ->
-    isEtaExp Σ b ->
-    unbox (ECSubst.csubst a k b) = ECSubst.csubst (unbox a) k (unbox b).
+  Lemma unbox_iota_red Σ pars args br :
+    unbox Σ (iota_red pars args br) = iota_red pars (map (unbox Σ) args) (on_snd (unbox Σ) br).
   Proof using Type.
-    intros cla etaa; move cla before a. move etaa before a.
-    funelim (unbox b); cbn; simp unbox isEtaExp; rewrite -?isEtaExp_equation_1 -?unbox_equation_1; toAll; simpl;
-    intros; try easy;
-    rewrite -> ?map_map_compose, ?compose_on_snd, ?compose_map_def, ?length_map;
-    unfold test_def in *;
-    simpl closed in *; try solve [simpl subst; simpl closed; f_equal; auto; rtoProp; solve_all]; try easy.
-
-    - destruct Nat.compare => //.
-    - f_equal. rtoProp. solve_all. destruct args; inv H0. eauto.
-    - f_equal. solve_all.  move/andP: b => [] _ he. solve_all.
-    - specialize (H a etaa cla k).
-      rewrite !csubst_mkApps in H1 *.
-      rewrite isEtaExp_mkApps_napp // in H1.
-      destruct construct_viewc.
-      * cbn. rewrite unbox_mkApps //.
-      * move/andP: H1 => [] et ev.
-        rewrite -H //.
-        assert (map (csubst a k) v <> []).
-        { destruct v; cbn; congruence. }
-        pose proof (etaExp_csubst Σ _ k _ etaa et).
-        destruct (isApp (csubst a k t)) eqn:eqa.
-        { destruct (decompose_app (csubst a k t)) eqn:eqk.
-          rewrite (decompose_app_inv eqk) in H2 *.
-          pose proof (decompose_app_notApp _ _ _ eqk).
-          assert (l <> []).
-          { intros ->. rewrite (decompose_app_inv eqk) in eqa. now rewrite eqa in H3. }
-          rewrite isEtaExp_mkApps_napp // in H2.
-          assert ((l ++ map (csubst a k) v)%list <> []).
-          { destruct l; cbn; congruence. }
-
-          destruct (construct_viewc t0) eqn:hc.
-          { rewrite -mkApps_app /=.
-            rewrite unbox_mkApps // unbox_mkApps //.
-            cbn -[lookup_inductive_pars].
-            move/andP: H2 => [] ise hl.
-            unfold isEtaExp_app in ise.
-            destruct is_unboxable eqn:isunb => //.
-            destruct l => //=.
-            rewrite (lookup_inductive_pars_constructor_pars_args eqpars).
-            rewrite -mkApps_app /= !skipn_map. f_equal.
-            rewrite skipn_app map_app. f_equal.
-            assert (pars - #|l| = 0). rtoProp. rename H2 into ise. eapply Nat.leb_le in ise; lia.
-            rewrite H2 skipn_0.
-            rewrite !map_map_compose.
-            clear -etaa cla ev H0. solve_all. }
-          { rewrite -mkApps_app.
-            rewrite unbox_mkApps //. rewrite hc.
-            rewrite unbox_mkApps // hc -mkApps_app map_app //.
-            f_equal. f_equal.
-            rewrite !map_map_compose.
-            clear -etaa cla ev H0. solve_all. } }
-        { rewrite unbox_mkApps ?eqa //.
-          destruct (construct_viewc (csubst a k t)) eqn:eqc.
-          2:{ f_equal. rewrite !map_map_compose. clear -etaa cla ev H0. solve_all. }
-          simp isEtaExp in H2.
-          rewrite /isEtaExp_app in H2.
-          destruct lookup_constructor_pars_args as [[pars args]|] eqn:eqpars => // /=.
-          rewrite (lookup_inductive_pars_constructor_pars_args eqpars).
-          assert (pars = 0). rtoProp. eapply Nat.leb_le in H2. lia.
-          subst pars. rewrite skipn_0.
-          simp unbox; rewrite -unbox_equation_1.
-          { f_equal. rewrite !map_map_compose. clear -etaa cla ev H0. solve_all. } }
-    - pose proof (etaExp_csubst _ _ k _ etaa H0).
-      rewrite !csubst_mkApps /= in H1 *.
-      assert (map (csubst a k) v <> []).
-      { destruct v; cbn; congruence. }
-      rewrite unbox_mkApps //.
-      rewrite isEtaExp_Constructor // in H1.
-      move/andP: H1. rewrite length_map. move=> [] etaapp etav.
-      cbn -[lookup_inductive_pars].
-      unfold isEtaExp_app in etaapp.
-      rewrite GlobalContextMap.lookup_inductive_pars_spec in Heq.
-      rewrite Heq in etaapp *.
-      f_equal.
-      now destruct block_args; inv etav.
-      rewrite map_skipn. f_equal.
-      rewrite !map_map_compose.
-      rewrite isEtaExp_Constructor // in H0. rtoProp. solve_all.
-    - pose proof (etaExp_csubst _ _ k _ etaa H0).
-      rewrite !csubst_mkApps /= in H1 *.
-      assert (map (csubst a k) v <> []).
-      { destruct v; cbn; congruence. }
-      rewrite unbox_mkApps //.
-      rewrite isEtaExp_Constructor // in H1.
-      rewrite GlobalContextMap.lookup_inductive_pars_spec in Heq.
-      move/andP: H1. rewrite length_map. move=> [] etaapp etav.
-      cbn -[lookup_inductive_pars].
-      unfold isEtaExp_app in etaapp.
-      destruct lookup_constructor_pars_args as [[pars args]|] eqn:eqpars => //.
-      now rewrite (lookup_inductive_pars_constructor_pars_args eqpars) in Heq.
-  Qed.
-
-  Lemma unbox_substl s t :
-    forallb (closedn 0) s ->
-    forallb (isEtaExp Σ) s ->
-    isEtaExp Σ t ->
-    unbox (substl s t) = substl (map unbox s) (unbox t).
-  Proof using Type.
-    induction s in t |- *; simpl; auto.
-    move=> /andP[] cla cls /andP[] etaa etas etat.
-    rewrite IHs //. now eapply etaExp_csubst. f_equal.
-    now rewrite unbox_csubst.
-  Qed.
-
-  Lemma unbox_iota_red pars args br :
-    forallb (closedn 0) args ->
-    forallb (isEtaExp Σ) args ->
-    isEtaExp Σ br.2 ->
-    unbox (EGlobalEnv.iota_red pars args br) = EGlobalEnv.iota_red pars (map unbox args) (on_snd unbox br).
-  Proof using Type.
-    intros cl etaargs etabr.
-    unfold EGlobalEnv.iota_red.
+    unfold iota_red.
+    simple.
     rewrite unbox_substl //.
-    rewrite forallb_rev forallb_skipn //.
-    rewrite forallb_rev forallb_skipn //.
-    now rewrite map_rev map_skipn.
   Qed.
 
-  Lemma unbox_fix_subst mfix : EGlobalEnv.fix_subst (map (map_def unbox) mfix) = map unbox (EGlobalEnv.fix_subst mfix).
+  (* Lemma unbox_fix_subst mfix : EGlobalEnv.fix_subst (map (map_def unbox) mfix) = map unbox (EGlobalEnv.fix_subst mfix).
   Proof using Type.
     unfold EGlobalEnv.fix_subst.
     rewrite length_map.
     generalize #|mfix|.
     induction n; simpl; auto.
-    f_equal; auto. now simp unbox.
+    f_equal; auto.
   Qed.
 
   Lemma unbox_cofix_subst mfix : EGlobalEnv.cofix_subst (map (map_def unbox) mfix) = map unbox (EGlobalEnv.cofix_subst mfix).
@@ -328,7 +1218,7 @@ Section unbox.
     rewrite length_map.
     generalize #|mfix|.
     induction n; simpl; auto.
-    f_equal; auto. now simp unbox.
+    f_equal; auto.
   Qed.
 
   Lemma unbox_cunfold_fix mfix idx n f :
@@ -373,13 +1263,12 @@ Section unbox.
     unbox (nth n l d) = nth n (map unbox l) (unbox d).
   Proof using Type.
     induction l in n |- *; destruct n; simpl; auto.
-  Qed.
+  Qed. *)
 
-  *)
 
 End unbox.
 
-#[universes(polymorphic)] Global Hint Rewrite @map_primIn_spec @map_InP_spec : unbox.
+(* #[universes(polymorphic)] Global Hint Rewrite @map_primIn_spec @map_InP_spec : unbox.
 Tactic Notation "simp_eta" "in" hyp(H) := simp isEtaExp in H; rewrite -?isEtaExp_equation_1 in H.
 Ltac simp_eta := simp isEtaExp; rewrite -?isEtaExp_equation_1.
 Tactic Notation "simp_unbox" "in" hyp(H) := simp unbox in H; rewrite -?unbox_equation_1 in H.
@@ -399,9 +1288,6 @@ Definition unbox_decl Σ d :=
 
 Definition unbox_env Σ :=
   map (on_snd (unbox_decl Σ)) Σ.(GlobalContextMap.global_decls).
-
-Definition unbox_program (p : eprogram_env) : eprogram :=
-  (unbox_env p.1, unbox p.1 p.2).
 
 Import EGlobalEnv.
 
@@ -520,7 +1406,6 @@ Proof.
   now rewrite remove_last_app.
 Qed.
 
-(*
 Arguments lookup_inductive_pars_constructor_pars_args {Σ ind n pars args}.
 
 Lemma unbox_tApp {Σ : GlobalContextMap.t} f a : isEtaExp Σ f -> isEtaExp Σ a -> unbox Σ (EAst.tApp f a) = EAst.tApp (unbox Σ f) (unbox Σ a).
@@ -530,8 +1415,8 @@ Proof.
   forward H by eauto.
   move/isEtaExp_mkApps: H.
   destruct decompose_app eqn:da.
-  destruct construct_viewc eqn:cv => //.
-  { intros [? [? []]]. rewrite H0 /=.
+  destruct construct_viewc eqn:cv => //. *)
+  (* { intros [? [? []]]. rewrite H0 /=.
     rewrite -[EAst.tApp _ _ ](mkApps_app _ _ [a]).
     move/andP: H2 => []. rewrite /isEtaExp_app.
     rewrite !unbox_mkApps // cv.
@@ -559,9 +1444,9 @@ Proof.
     assert (l <> []).
     { destruct l; try congruence. eapply decompose_app_inv in da. cbn in *. now subst t. }
     rewrite H1.
-    now apply remove_last_last. }
-Qed.
-
+    now apply remove_last_last. } 
+Qed.*)
+(*
 Module Fast.
   Section fastunbox.
     Context (Σ : GlobalContextMap.t).
